thys/cost/Enat_Cost.thy
@@ -9,5 +9,7 @@ declare [[coercion_enabled = false]]
 definition "lift_acost c \<equiv> acostC (enat o the_acost c)"
 
 
+lemma lift_acost_cost: "lift_acost (cost name x) = (cost name (enat x))"
+  by (auto simp: one_enat_def zero_enat_def lift_acost_def cost_def zero_acost_def)
 
 end
